\documentclass{article}

\usepackage{amsmath}
\usepackage{ amssymb } 

\begin{document}
	{\Large \textbf{Math 1 Answers} - \textit{Chapter Two}}
	
	\begin{enumerate}
		\item 
		
		\item 
		
		\item 
		
		\item 
		\begin{align*}
			\lim_{x \rightarrow 1} \frac{\ln x}{x - 1} = \frac{0}{0} \\
			\underrightarrow{Hopital} \lim_{x \rightarrow 1} \frac{\frac{1}{x}}{1} = 1 = f(1)		
		\end{align*}
	
		So $f(x)$ is continues in $x = 1$.
		
		\item We must show the function is derivative in $x = 0$
		\begin{align*}
			\lim_{x \rightarrow 0} \frac{f(x) - f(0)}{x - 0} &= \lim_{x \rightarrow 0} \frac{x^2\sin\frac{1}{x}}{x} \\
			&= \lim_{x \rightarrow 0} x\sin\frac{1}{x} = 0
		\end{align*}
		And $f'(x)$ equal to:
		\begin{align*}
			f'(x) &= 2x\sin\frac{1}{x} + x^2\frac{1}{x^2}\cos\frac{1}{x} \\
			&= 2x\sin\frac{1}{x} - \cos\frac{1}{x} 
		\end{align*}
	
		Part B:
		\begin{align*}
			\lim_{x \rightarrow 0} f'(x) &= \lim_{x \rightarrow 0} 2x\sin\frac{1}{x} - \cos\frac{1}{x} \\
			&= \lim_{x \rightarrow 0} -\cos x = -1 \neq f'(0)
		\end{align*}
	
		\item 
		
		\item A) Deform equation to:
		\begin{align*}
			f(x) = \frac{f(x + y)}{f(y)}
		\end{align*}
		Calculate $x = 0$:
		\begin{align*}
			f(0) = \frac{f(0 + y)}{f(y)} = 1 (f(y) \neq 0)
		\end{align*}
	
		B)
		
		\item
		\begin{align*}
			\underrightarrow{Hopital} \lim_{x \rightarrow a} \frac{f(a) - 0 - af'(x))}{1} = f(a) - af'(x)
		\end{align*}
	
		\item 
		\begin{align*}
			g'(x) = \frac{\cos x}{2\sqrt{\sin x}} + \frac{1}{2\sqrt{x}}\cos\sqrt{x} \\
			g''(x) = 
		\end{align*}
	
		\item A)
		\begin{align*}
			h'(x) &= \frac{f'(x)g(x) - f(x)g'(x)}{g^2(x)} \\
			&= \frac{2 - 0}{4} \\
			&= \frac{1}{2}
		\end{align*}
	
		B)
		\begin{align*}
			h'(x) &= \frac{g'(x)(1 + f(x)) - g(x)f'(x)}{(1 + f(x)) \times 2} \\
			&= \frac{1}{2}
		\end{align*}
	
		C)
		\begin{align*}
			h'(t) &= \frac{(f(t) + g(t)) - t(f'(t) + g'(t))}{(f(t) + g(t))^2} \\
			&= \frac{3 - 1}{3^2} = 9
		\end{align*}
	
		\item 
		
		\item $f(x)$ is derivative, so it is continues in $x = 2$:
		\begin{align*}
			\lim_{x \rightarrow 2^+} 2a + b = \lim_{x \rightarrow 2^-} 4 = f(2) = 4
		\end{align*}
		So:
		\begin{align*}
			a = 4 \\
			2a + b = 4 \rightarrow b = -4 \\
			f'(x) = \text{if} x \leqslant 2 \text{then} 2x | \text{if} x \textgreater 2 \text{then} 4	
		\end{align*}
		*BUG
		
		\item 
		
		\item 
		\begin{align*}
			F'(x) = (f(x) - xf'(x))(f'(xf(x))) \\
			F'(0) = 1 \times 2 = 2
		\end{align*}
	
		\item
		
		\item
		
		\item
		\begin{align*}
			(f(g(x)))' &= 1 \\
			&= g'(x)f'(g(x)) \\
			&= g'(x)(1 + g^2(x)) = 1 \\
		\end{align*}
		So:
		\begin{align*}
			g'(x) = \frac{1}{1 + g^2(x)}
		\end{align*}
			
		\item 
		\begin{align*}
			\lim_{x \rightarrow a} \frac{f'(x)}{\frac{1}{2\sqrt{x}}} &= \lim_{x \rightarrow a} 2\sqrt{x}f'(x) \\
			&= 2\sqrt{a}f'(a)
		\end{align*}
	
		\item 
		
		\item 
		
	
					
	\end{enumerate}

\end{document}